wip

Logic/Propositional/Superintuitionistic/Kripke/Semantics.lean
@@ -1,9 +1,221 @@
 import Logic.Vorspiel.BinaryRelations
 import Logic.Logic.Semantics
-import Logic.Propositional.Superintuitionistic.Formula
+import Logic.Propositional.Superintuitionistic.Deduction
+
+namespace LO.Kripke
+
+structure Frame where
+  World : Type*
+  Rel : Rel World World
+  [World_nonempty : Nonempty World]
+
+instance : CoeSort Frame Type* := ⟨Frame.World⟩
+instance : CoeFun Frame (λ F => F.World → F.World → Prop) := ⟨Frame.Rel⟩
+
+instance {F : Frame} : Nonempty F.World := F.World_nonempty
+
+abbrev Frame.Rel' {F : Frame} (x y : F.World) := F.Rel x y
+scoped infix:45 " ≺ " => Frame.Rel'
+
+noncomputable abbrev Frame.default {F : Frame} : F.World := Classical.choice F.World_nonempty
+notation "﹫" => Frame.default
+
+
+set_option linter.unusedVariables false in
+abbrev Frame.Dep (α : Type*) := Frame
+
+abbrev Frame.alt (F : Frame) {α} : Frame.Dep α := F
+scoped postfix:max "#" => Frame.alt
+
+
+structure FiniteFrame extends Frame where
+  [World_finite : Finite World]
+
+instance {F : FiniteFrame} : Finite (F.World) := F.World_finite
+instance : Coe (FiniteFrame) (Frame) := ⟨λ F ↦ F.toFrame⟩
+
+
+open Relation (ReflTransGen TransGen)
+
+
+protected abbrev Frame.RelReflTransGen {F : Frame} : _root_.Rel F.World F.World:= ReflTransGen (· ≺ ·)
+scoped infix:45 " ≺^* " => Frame.RelReflTransGen
+
+namespace Frame.RelReflTransGen
+
+variable {F : Frame}
+
+@[simp] lemma single {x y : F.World} (hxy : x ≺ y) : x ≺^* y := ReflTransGen.single hxy
+
+@[simp] lemma reflexive : Reflexive F.RelReflTransGen := Relation.reflexive_reflTransGen
+
+@[simp] lemma refl {x : F.World} : x ≺^* x := reflexive x
+
+@[simp] lemma transitive : Transitive F.RelReflTransGen := Relation.transitive_reflTransGen
+
+@[simp] lemma symmetric : Symmetric F.Rel → Symmetric F.RelReflTransGen := ReflTransGen.symmetric
+
+end Frame.RelReflTransGen
+
+
+abbrev Frame.TransitiveReflexiveClosure (F : Frame) : Frame where
+  World := F.World
+  Rel := (· ≺^* ·)
+postfix:max "^*" => Frame.TransitiveReflexiveClosure
+
+namespace Frame.TransitiveReflexiveClosure
+
+variable {F : Frame}
+
+lemma single {x y : F.World} (hxy : x ≺ y) : F^*.Rel x y := ReflTransGen.single hxy
+
+lemma rel_reflexive : Reflexive F^*.Rel := by intro x; exact ReflTransGen.refl;
+
+lemma rel_transitive : Transitive F^*.Rel := by simp;
+
+lemma rel_symmetric : Symmetric F.Rel → Symmetric F^* := ReflTransGen.symmetric
+
+end Frame.TransitiveReflexiveClosure
+
+
+
+protected abbrev Frame.RelTransGen {F : Frame} : _root_.Rel F.World F.World := TransGen (· ≺ ·)
+scoped infix:45 " ≺^+ " => Frame.RelTransGen
+
+namespace Frame.RelTransGen
+
+variable {F : Frame}
+
+@[simp] lemma single {x y : F.World} (hxy : x ≺ y) : x ≺^+ y := TransGen.single hxy
+
+@[simp]
+lemma transitive : Transitive F.RelTransGen := λ _ _ _ => TransGen.trans
+
+@[simp]
+lemma symmetric (hSymm : Symmetric F.Rel) : Symmetric F.RelTransGen := by
+  intro x y rxy;
+  induction rxy with
+  | single h => exact TransGen.single $ hSymm h;
+  | tail _ hyz ih => exact TransGen.trans (TransGen.single $ hSymm hyz) ih
+
+end Frame.RelTransGen
+
+
+abbrev Frame.TransitiveClosure (F : Frame) : Frame where
+  World := F.World
+  Rel := (· ≺^+ ·)
+scoped postfix:max "^+" => Frame.TransitiveClosure
+
+namespace Frame.TransitiveClosure
+
+variable {F : Frame}
+
+lemma single {x y : F.World} (hxy : x ≺ y) : F^+ x y := TransGen.single hxy
+
+lemma rel_transitive : Transitive F^+ := by simp;
+
+lemma rel_symmetric (hSymm : Symmetric F.Rel) : Symmetric F.TransitiveClosure := by simp_all
+
+end Frame.TransitiveClosure
+
+
+abbrev FrameProperty := Frame → Prop
+
+
+abbrev FrameClass := Set (Frame)
+
+set_option linter.unusedVariables false in
+abbrev FrameClass.Dep (α : Type*) := FrameClass
+
+abbrev FrameClass.alt (𝔽 : FrameClass) {α} : FrameClass.Dep α := 𝔽
+scoped postfix:max "#" => FrameClass.alt
+
+
+abbrev FiniteFrameClass := Set (FiniteFrame)
+
+@[simp] def FiniteFrameClass.toFrameClass (𝔽 : FiniteFrameClass) : FrameClass := { F | ∃ F', F' ∈ 𝔽 ∧ F'.toFrame = F }
+instance : Coe (FiniteFrameClass) (FrameClass) := ⟨FiniteFrameClass.toFrameClass⟩
+
+@[simp] def FrameClass.toFiniteFrameClass (𝔽 : FrameClass) : FiniteFrameClass := { F | F.toFrame ∈ 𝔽 }
+instance : Coe (FrameClass) (FiniteFrameClass) := ⟨FrameClass.toFiniteFrameClass⟩
+
+@[simp] abbrev FrameClass.restrictFinite (𝔽 : FrameClass) : FrameClass := FiniteFrameClass.toFrameClass ↑𝔽
+postfix:max "ꟳ" => FrameClass.restrictFinite
+
+lemma FrameClass.iff_mem_restrictFinite {𝔽 : FrameClass} (h : F ∈ 𝔽) (F_finite : Finite F.World) : F ∈ 𝔽ꟳ := by
+  simp;
+  use { toFrame := F, World_finite := F_finite };
+
+
+abbrev FrameClassOfSystem [System F S] [Semantics F (Frame.Dep α)] (𝓢 : S) : FrameClass.Dep α := { (F : Frame.Dep α) | F ⊧* System.theory 𝓢 }
+notation "𝔽(" 𝓢 ")" => FrameClassOfSystem 𝓢
+
+abbrev FrameClassOfFrameProperty (P : FrameProperty) : FrameClass := { F | P F }
+notation "𝔽(" P ")" => FrameClassOfFrameProperty P
+
+
+class Characteraizable (𝔽 : FrameClass) (P : FrameProperty) where
+  characterize : ∀ {F}, P F → F ∈ 𝔽
+  nonempty : ∃ F, P F
+
+
+section Soundness
+
+variable [System F S] [Semantics F (Frame.Dep α)] {𝓢 : S}
+
+lemma sound : 𝓢 ⊢! p → (FrameClassOfSystem (α := α) 𝓢) ⊧ p := by
+  intro hp F hF;
+  simp [System.theory] at hF;
+  exact hF p hp;
+
+instance : Sound 𝓢 (FrameClassOfSystem (α := α) 𝓢) := ⟨sound⟩
+
+
+lemma sound_of_characterizability (characterizability : Characteraizable (FrameClassOfSystem (α := α) 𝓢) P) : 𝓢 ⊢! p → 𝔽(P) ⊧ p := by
+  intro h F hF;
+  apply sound h;
+  apply characterizability.characterize hF;
+
+instance instSoundOfCharacterizability (characterizability : Characteraizable (FrameClassOfSystem (α := α) 𝓢) P)
+  : Sound 𝓢 (FrameClassOfFrameProperty P) := ⟨sound_of_characterizability characterizability⟩
+
+
+variable [LogicalConnective F] [Semantics.Bot (FrameClass.Dep α)]
+
+lemma unprovable_bot : 𝓢 ⊬! ⊥ := by
+  apply (not_imp_not.mpr (sound (α := α)));
+  exact Semantics.Bot.realize_bot 𝔽(𝓢);
+
+lemma unprovable_bot_of_characterizability [characterizability : Characteraizable (FrameClassOfSystem (α := α) 𝓢) P] : 𝓢 ⊬! ⊥ := by
+  apply not_imp_not.mpr $ sound_of_characterizability (characterizability := characterizability);
+  exact Semantics.Bot.realize_bot 𝔽(P);
+
+-- instance : System.Consistent 𝓢 := System.Consistent.of_unprovable $ unprovable_bot (α := α)
+
+end Soundness
+
+
+abbrev Valuation (F : Frame) (α : Type*) := F.World → α → Prop
+
+def Valuation.atomic_hereditary (V : Valuation F α) : Prop := ∀ {w₁ w₂ : F.World}, (w₁ ≺ w₂) → ∀ {a}, (V w₁ a) → (V w₂ a)
+  -- (atom_hereditary : ∀ {w₁ w₂ : M.World}, (w₁ ≺ w₂) → ∀ {a}, (M.Valuation w₁ a) → (M.Valuation w₂ a))
+  -- (F_trans : Transitive M.Frame.Rel)
+  -- (F_refl : Reflexive M.Frame.Rel)
+
+
+structure Model (α) where
+  Frame : Frame
+  Valuation : Valuation Frame α
+
+abbrev Model.World (M : Model α) := M.Frame.World
+instance : CoeSort (Model α) (Type u) := ⟨Model.World⟩
+
+end LO.Kripke
+
 
 namespace LO.Propositional.Superintuitionistic
 
+/-
 namespace Kripke
 
 attribute [simp] Reflexive Transitive Antisymmetric in
@@ -82,6 +294,7 @@ section
 end
 
 end Kripke
+-/
 
 open System
 open Kripke
@@ -94,8 +307,8 @@ def Formula.Kripke.Satisfies (M : Kripke.Model α) (w : M.World) : Formula α �
   | ⊥      => False
   | p ⋏ q  => Satisfies M w p ∧ Satisfies M w q
   | p ⋎ q  => Satisfies M w p ∨ Satisfies M w q
-  | ~p     => ∀ {w'}, (w ≺ w') → ¬Satisfies M w' p
-  | p ⟶ q => ∀ {w'}, (w ≺ w') → (Satisfies M w' p → Satisfies M w' q)
+  | ~p     => ∀ {w' : M.World}, (w ≺ w') → ¬Satisfies M w' p
+  | p ⟶ q => ∀ {w' : M.World}, (w ≺ w') → (Satisfies M w' p → Satisfies M w' q)
 
 instance instKripkeSemanticsFormulaWorld (M : Model α) : Semantics (Formula α) (M.World) := ⟨fun w ↦ Formula.Kripke.Satisfies M w⟩
 
@@ -103,19 +316,17 @@ open Formula.Kripke
 
 namespace Formula.Kripke.Satisfies
 
-variable {M : Model α}
+variable {M : Model α} {w : M.World} {p q r : Formula α}
 
 @[simp] protected lemma iff_models : w ⊧ p ↔ Formula.Kripke.Satisfies M w p := iff_of_eq rfl
 
-local infix:45 " ⊩ " => Formula.Kripke.Satisfies M
-
-@[simp] lemma atom_def : w ⊩ atom a ↔ M.Valuation w a := by simp [Satisfies];
-@[simp] lemma top_def  : w ⊩ ⊤ ↔ True := by simp [Satisfies];
-@[simp] lemma bot_def  : w ⊩ ⊥ ↔ False := by simp [Satisfies];
-@[simp] lemma and_def  : w ⊩ p ⋏ q ↔ w ⊩ p ∧ w ⊩ q := by simp [Satisfies];
-@[simp] lemma or_def   : w ⊩ p ⋎ q ↔ w ⊩ p ∨ w ⊩ q := by simp [Satisfies];
-@[simp] lemma imp_def  : w ⊩ p ⟶ q ↔ ∀ {w'}, (w ≺ w') → (w' ⊩ p → w' ⊩ q) := by simp [Satisfies, imp_iff_not_or];
-@[simp] lemma neg_def  : w ⊩ ~p ↔ ∀ {w'}, (w ≺ w') → ¬(w' ⊩ p) := by simp [Satisfies];
+@[simp] lemma atom_def : w ⊧ atom a ↔ M.Valuation w a := by simp [Satisfies];
+@[simp] lemma top_def  : w ⊧ ⊤ ↔ True := by simp [Satisfies];
+@[simp] lemma bot_def  : w ⊧ ⊥ ↔ False := by simp [Satisfies];
+@[simp] lemma and_def  : w ⊧ p ⋏ q ↔ w ⊧ p ∧ w ⊧ q := by simp [Satisfies];
+@[simp] lemma or_def   : w ⊧ p ⋎ q ↔ w ⊧ p ∨ w ⊧ q := by simp [Satisfies];
+@[simp] lemma imp_def  : w ⊧ p ⟶ q ↔ ∀ {w' : M.World}, (w ≺ w') → (w' ⊧ p → w' ⊧ q) := by simp [Satisfies, imp_iff_not_or];
+@[simp] lemma neg_def  : w ⊧ ~p ↔ ∀ {w' : M.World}, (w ≺ w') → ¬(w' ⊧ p) := by simp [Satisfies];
 
 instance : Semantics.Top M.World where
   realize_top := by simp [Satisfies];
@@ -129,17 +340,20 @@ instance : Semantics.And M.World where
 instance : Semantics.Or M.World where
   realize_or := by simp [Satisfies];
 
-lemma formula_hereditary (hw : w ≺ w') : w ⊩ p → w' ⊩ p := by
+
+
+lemma formula_hereditary
+  (herditary : M.Valuation.atomic_hereditary)
+  (F_trans : Transitive M.Frame.Rel)
+  (hw : w ≺ w') : w ⊧ p → w' ⊧ p := by
   induction p using Formula.rec' with
-  | hatom => apply M.hereditary hw;
+  | hatom => apply herditary hw;
   | himp =>
-    simp_all [Satisfies];
     intro hpq v hv;
-    exact hpq $ M.Frame.Rel_trans hw hv;
+    exact hpq $ F_trans hw hv;
   | hneg =>
-    simp_all [Satisfies];
     intro hp v hv;
-    exact hp $ M.Frame.Rel_trans hw hv;
+    exact hp $ F_trans hw hv;
   | hor => simp_all [Satisfies]; tauto;
   | _ => simp_all [Satisfies];
 
@@ -148,60 +362,65 @@ lemma hereditary_int {M : Model (𝐈𝐧𝐭 W α)} {w w' : W} {p : Formula α}
   apply hereditary (by simp [FrameClass.Intuitionistic]; tauto) hw;
 -/
 
-lemma neg_equiv : w ⊩ ~p ↔ w ⊩ p ⟶ ⊥ := by simp_all [Satisfies];
+lemma neg_equiv : w ⊧ ~p ↔ w ⊧ p ⟶ ⊥ := by simp_all [Satisfies];
 
 end Formula.Kripke.Satisfies
 
 
-def Formula.Kripke.ValidOnModel (M : Model α) (p : Formula α) := ∀ w : M.World, w ⊧ p
+open Formula.Kripke.Satisfies (formula_hereditary)
 
-instance : Semantics (Formula α) (Model α) := ⟨fun M ↦ Formula.Kripke.ValidOnModel M⟩
+
+def Formula.Kripke.ValidOnModel (M : Model α) (p : Formula α) := ∀ w : M.World, w ⊧ p
 
 namespace Formula.Kripke.ValidOnModel
 
-@[simp] protected lemma iff_models : M ⊧ p ↔ Formula.Kripke.ValidOnModel M p := iff_of_eq rfl
+variable
+  {M : Model α} {p q r : Formula α}
+  (atom_hereditary : ∀ {w₁ w₂ : M.World}, (w₁ ≺ w₂) → ∀ {a}, (M.Valuation w₁ a) → (M.Valuation w₂ a))
+  (F_trans : Transitive M.Frame.Rel := by simpa)
+  (F_refl : Reflexive M.Frame.Rel := by simpa)
 
--- variable {𝔽 : FrameClass W α} (hTrans : 𝔽 ⊆ { F | Transitive F }) (hRefl : 𝔽 ⊆ { F | Reflexive F })
-variable {M : Model α} {p q r : Formula α}
+instance : Semantics (Formula α) (Model α) := ⟨fun M ↦ Formula.Kripke.ValidOnModel M⟩
+
+@[simp] protected lemma iff_models : M ⊧ p ↔ Formula.Kripke.ValidOnModel M p := iff_of_eq rfl
 
 @[simp] protected lemma verum : M ⊧ ⊤ := by simp_all [ValidOnModel];
 
-@[simp] protected lemma and₁ : M ⊧ p ⋏ q ⟶ p := by simp_all [ValidOnModel];
+@[simp] protected lemma and₁ : M ⊧ p ⋏ q ⟶ p := by simp_all [ValidOnModel, Satisfies];
 
-@[simp] protected lemma and₂ : M ⊧ p ⋏ q ⟶ q := by simp_all [ValidOnModel];
+@[simp] protected lemma and₂ : M ⊧ p ⋏ q ⟶ q := by simp_all [ValidOnModel, Satisfies];
 
 @[simp] protected lemma and₃ : M ⊧ p ⟶ q ⟶ p ⋏ q := by
-  simp_all [ValidOnModel];
-  intro w₁ w₂ _ hp w₃ hw₂₃ _;
-  exact Satisfies.formula_hereditary hw₂₃ hp;
+  intro x y _ hp z Ryz hq;
+  replace hp : Satisfies M z p := formula_hereditary atom_hereditary F_trans Ryz hp;
+  exact ⟨hp, hq⟩;
 
-@[simp] protected lemma or₁ : M ⊧ p ⟶ p ⋎ q := by simp_all [ValidOnModel];
+@[simp] protected lemma or₁ : M ⊧ p ⟶ p ⋎ q := by simp_all [ValidOnModel, Satisfies];
 
-@[simp] protected lemma or₂ : M ⊧ q ⟶ p ⋎ q := by simp_all [ValidOnModel];
+@[simp] protected lemma or₂ : M ⊧ q ⟶ p ⋎ q := by simp_all [ValidOnModel, Satisfies];
 
 @[simp] protected lemma or₃ : M ⊧ (p ⟶ r) ⟶ (q ⟶ r) ⟶ (p ⋎ q ⟶ r) := by
   simp_all only [ValidOnModel.iff_models, ValidOnModel, Satisfies.iff_models, Satisfies.imp_def, Satisfies.or_def];
   intro w₁ w₂ _ hpr w₃ hw₂₃ hqr w₄ hw₃₄ hpq;
   cases hpq with
-  | inl hp => exact hpr (M.Frame.Rel_trans hw₂₃ hw₃₄) hp;
+  | inl hp => exact hpr (F_trans hw₂₃ hw₃₄) hp;
   | inr hq => exact hqr hw₃₄ hq;
 
 @[simp] protected lemma imply₁ : M ⊧ p ⟶ q ⟶ p := by
-  simp_all [ValidOnModel];
-  intro w₁ w₂ _ hp w₃ hw₂₃ _;
-  exact Satisfies.formula_hereditary hw₂₃ hp;
+  intro x y _ hp z Ryz _;
+  exact formula_hereditary atom_hereditary F_trans Ryz hp;
 
 @[simp] protected lemma imply₂ : M ⊧ (p ⟶ q ⟶ r) ⟶ (p ⟶ q) ⟶ p ⟶ r := by
-  simp_all only [ValidOnModel.iff_models, ValidOnModel, Satisfies.iff_models, Satisfies.imp_def];
-  intro w₁ w₂ _ hpqr w₃ hw₂₃ hpq w₄ hw₃₄ hp;
-  exact hpqr (M.Frame.Rel_trans hw₂₃ hw₃₄) hp (M.Frame.Rel_refl w₄) (hpq hw₃₄ hp);
+  intro x y _ hpqr z Ryz hpq w Rzw hp;
+  have Ryw := F_trans Ryz Rzw;
+  have Rww := F_refl w;
+  exact hpqr Ryw hp Rww (hpq Rzw hp);
 
 @[simp] protected lemma mdp (hpq : M ⊧ p ⟶ q) (hp : M ⊧ p) : M ⊧ q := by
-  simp_all [ValidOnModel];
   intro w;
-  exact hpq _ (M.Frame.Rel_refl w);
+  exact hpq w (F_refl w) $ hp w;
 
-@[simp] protected lemma efq : M ⊧ Axioms.EFQ p := by simp_all [ValidOnModel];
+@[simp] protected lemma efq : M ⊧ Axioms.EFQ p := by simp [ValidOnModel, Satisfies];
 
 @[simp] protected lemma neg_equiv : M ⊧ Axioms.NegEquiv p := by
   simp_all [ValidOnModel, Axioms.NegEquiv];
@@ -210,7 +429,7 @@ variable {M : Model α} {p q r : Formula α}
   . intro x _ h y rxy hyp; exact h rxy hyp;
   . intro x _ h y rxy; exact h rxy;
 
-@[simp] protected lemma lem (hExt : Extensive M.Rel) : M ⊧ Axioms.LEM p := by
+@[simp] protected lemma lem (hExt : Extensive M.Frame.Rel) : M ⊧ Axioms.LEM p := by
   simp_all [ValidOnModel];
   intro w;
   by_cases h : w ⊧ p
@@ -223,89 +442,72 @@ variable {M : Model α} {p q r : Formula α}
 end Formula.Kripke.ValidOnModel
 
 
-def Formula.Kripke.ValidOnFrame (F : Frame) (p : Formula α) := ∀ (V : Valuation F.World α), (h : _) → (Model.mk F V h) ⊧ p
-
-instance : Semantics (Formula α) (Frame' α) := ⟨fun F ↦ Formula.Kripke.ValidOnFrame F⟩
+def Formula.Kripke.ValidOnFrame (F : Frame) (p : Formula α) := ∀ {V : Valuation F α}, {_ : V.atomic_hereditary} → (⟨F, V⟩ : Kripke.Model α) ⊧ p
 
 namespace Formula.Kripke.ValidOnFrame
 
-@[simp] protected lemma models_iff {F : Frame' α} : F ⊧ f ↔ ValidOnFrame F f := iff_of_eq rfl
+instance : Semantics (Formula α) (Frame.Dep α) := ⟨fun F ↦ Formula.Kripke.ValidOnFrame F⟩
 
+variable {F : Frame.Dep α}
 
-variable {F : Frame' α} {p q r : Formula α}
+@[simp] protected lemma models_iff : F ⊧ f ↔ ValidOnFrame F f := iff_of_eq rfl
 
-@[simp] protected lemma verum : F ⊧ ⊤ := by
-  simp_all only [ValidOnFrame.models_iff, ValidOnFrame, ValidOnModel.iff_models];
-  intros; apply ValidOnModel.verum;
+variable {F : Frame.Dep α} {p q r : Formula α}
+         (F_trans : Transitive F)
+         (F_refl : Reflexive F)
 
-@[simp] protected lemma and₁ : F ⊧ p ⋏ q ⟶ p := by
-  simp_all only [ValidOnFrame.models_iff, ValidOnFrame, ValidOnModel.iff_models];
-  intros; apply ValidOnModel.and₁;
+@[simp] protected lemma verum : F ⊧ ⊤ := ValidOnModel.verum
 
-@[simp] protected lemma and₂ : F ⊧ p ⋏ q ⟶ q := by
-  simp_all only [ValidOnFrame.models_iff, ValidOnFrame, ValidOnModel.iff_models];
-  intros; apply ValidOnModel.and₂;
+@[simp] protected lemma and₁ : F ⊧ p ⋏ q ⟶ p := ValidOnModel.and₁
 
-@[simp] protected lemma and₃ : F ⊧ p ⟶ q ⟶ p ⋏ q := by
-  simp_all only [ValidOnFrame.models_iff, ValidOnFrame, ValidOnModel.iff_models];
-  intros; apply ValidOnModel.and₃;
+@[simp] protected lemma and₂ : F ⊧ p ⋏ q ⟶ q := ValidOnModel.and₂
 
-@[simp] protected lemma or₁ : F ⊧ p ⟶ p ⋎ q := by
-  simp_all only [ValidOnFrame.models_iff, ValidOnFrame, ValidOnModel.iff_models];
-  intros; apply ValidOnModel.or₁;
+@[simp] protected lemma and₃ : F ⊧ p ⟶ q ⟶ p ⋏ q := by intros _ hV; exact ValidOnModel.and₃ hV;
 
-@[simp] protected lemma or₂ : F ⊧ q ⟶ p ⋎ q := by
-  simp_all only [ValidOnFrame.models_iff, ValidOnFrame, ValidOnModel.iff_models];
-  intros; apply ValidOnModel.or₂;
+@[simp] protected lemma or₁ : F ⊧ p ⟶ p ⋎ q := ValidOnModel.or₁
 
-@[simp] protected lemma or₃ : F ⊧ (p ⟶ r) ⟶ (q ⟶ r) ⟶ (p ⋎ q ⟶ r) := by
-  simp_all only [ValidOnFrame.models_iff, ValidOnFrame, ValidOnModel.iff_models];
-  intros; apply ValidOnModel.or₃;
+@[simp] protected lemma or₂ : F ⊧ q ⟶ p ⋎ q := ValidOnModel.or₂
 
-@[simp] protected lemma imply₁ : F ⊧ p ⟶ q ⟶ p := by
-  simp_all only [ValidOnFrame.models_iff, ValidOnFrame, ValidOnModel.iff_models];
-  intros; apply ValidOnModel.imply₁;
+@[simp] protected lemma or₃ : F ⊧ (p ⟶ r) ⟶ (q ⟶ r) ⟶ (p ⋎ q ⟶ r) := ValidOnModel.or₃
 
-@[simp] protected lemma imply₂ : F ⊧ (p ⟶ q ⟶ r) ⟶ (p ⟶ q) ⟶ p ⟶ r := by
-  simp_all only [ValidOnFrame.models_iff, ValidOnFrame, ValidOnModel.iff_models];
-  intros; apply ValidOnModel.imply₂;
+@[simp] protected lemma imply₁ : F ⊧ p ⟶ q ⟶ p := by intros _ hV; exact ValidOnModel.imply₁ hV;
+
+@[simp] protected lemma imply₂ : F ⊧ (p ⟶ q ⟶ r) ⟶ (p ⟶ q) ⟶ p ⟶ r := ValidOnModel.imply₂
 
 @[simp] protected lemma mdp (hpq : F ⊧ p ⟶ q) (hp : F ⊧ p) : F ⊧ q := by
-  simp_all only [ValidOnFrame.models_iff, ValidOnFrame, ValidOnModel.iff_models];
   intros V hV;
-  exact ValidOnModel.mdp (hpq V hV) (hp V hV);
+  exact ValidOnModel.mdp (F_refl := F_refl) (@hpq V hV) (@hp V hV);
 
-@[simp] protected lemma efq : F ⊧ Axioms.EFQ p := by
-  simp_all only [ValidOnFrame.models_iff, ValidOnFrame, ValidOnModel.iff_models];
-  intros; apply ValidOnModel.efq;
+@[simp] protected lemma efq : F ⊧ Axioms.EFQ p := ValidOnModel.efq
 
-@[simp] protected lemma neg_equiv : F ⊧ Axioms.NegEquiv p := by
-  simp_all only [ValidOnFrame.models_iff, ValidOnFrame, ValidOnModel.iff_models];
-  intros; apply ValidOnModel.neg_equiv;
+@[simp] protected lemma neg_equiv : F ⊧ Axioms.NegEquiv p := ValidOnModel.neg_equiv
 
-@[simp] protected lemma lem (hExt : Extensive F.Rel) : F ⊧ Axioms.LEM p := by
-  simp_all only [ValidOnFrame.models_iff, ValidOnFrame, ValidOnModel.iff_models];
-  intros; exact ValidOnModel.lem hExt;
+@[simp] protected lemma lem (hExt : Extensive F.Rel) : F ⊧ Axioms.LEM p := ValidOnModel.lem hExt
 
-instance : Semantics.Bot (Frame' α) where
+instance : Semantics.Bot (Frame.Dep α) where
   realize_bot _ := by
     simp [ValidOnModel, ValidOnFrame];
     existsi (λ _ _ => True);
-    simp_all;
+    simp_all [Satisfies, Valuation.atomic_hereditary];
 
 end Formula.Kripke.ValidOnFrame
 
 
-@[simp] def Formula.Kripke.ValidOnFrameClass (𝔽 : FrameClass) (p : Formula α) := ∀ {F : Frame' α}, F ∈ 𝔽 → F ⊧ p
-
-instance : Semantics (Formula α) (FrameClass' α) := ⟨fun 𝔽 ↦ Formula.Kripke.ValidOnFrameClass 𝔽⟩
+@[simp] def Formula.Kripke.ValidOnFrameClass (𝔽 : FrameClass) (p : Formula α) := ∀ {F : Frame}, F ∈ 𝔽 → F# ⊧ p
 
 namespace Formula.Kripke.ValidOnFrameClass
 
-@[simp] protected lemma iff_models {𝔽 : FrameClass' α} : 𝔽 ⊧ p ↔ Formula.Kripke.ValidOnFrameClass 𝔽 p := iff_of_eq rfl
+instance : Semantics (Formula α) (FrameClass.Dep α) := ⟨fun 𝔽 ↦ Formula.Kripke.ValidOnFrameClass 𝔽⟩
+
+@[simp] protected lemma iff_models {𝔽 : FrameClass.Dep α} : 𝔽 ⊧ p ↔ Formula.Kripke.ValidOnFrameClass 𝔽 p := iff_of_eq rfl
+
+protected lemma realize_bot {𝔽 : FrameClass.Dep α} (ne : 𝔽.Nonempty) : ¬(𝔽 ⊧ ⊥) := by
+  simp [ValidOnFrameClass.iff_models, ValidOnFrameClass];
+  exact ne;
 
 end Formula.Kripke.ValidOnFrameClass
 
+/-
 @[simp] def Formula.Kripke.ValidOnFiniteFrameClass (𝔽 : FiniteFrameClass) (f : Formula α) := ∀ (F : FiniteFrame' α), F ∈ 𝔽 → F.toFrame' ⊧ f
 
 instance : Semantics (Formula α) (FiniteFrameClass' α) := ⟨fun 𝔽 ↦ Formula.Kripke.ValidOnFiniteFrameClass 𝔽⟩
@@ -315,24 +517,105 @@ namespace Formula.Kripke.ValidOnFiniteFrameClass
 @[simp] protected lemma models_iff {𝔽 : FiniteFrameClass' α} : 𝔽 ⊧ f ↔ Formula.Kripke.ValidOnFiniteFrameClass 𝔽 f := iff_of_eq rfl
 
 end Formula.Kripke.ValidOnFiniteFrameClass
+-/
 
 
 namespace Kripke
 
-def AxiomSetFrameClass (Ax : AxiomSet α) : FrameClass' α := { (F : Frame' α) | F ⊧* Ax }
+instance Characteraizable_Int : Kripke.Characteraizable 𝔽((𝐈𝐧𝐭 : DeductionParameter α)) (λ F => Transitive F ∧ Reflexive F) where
+  characterize := by
+    simp [System.theory];
+    intro F hTrans hRefl p hp;
+    induction hp using Deduction.rec! with
+    | verum => apply ValidOnFrame.verum;
+    | imply₁ => apply ValidOnFrame.imply₁; simpa;
+    | imply₂ => apply ValidOnFrame.imply₂; simpa; simpa;
+    | and₁ => apply ValidOnFrame.and₁;
+    | and₂ => apply ValidOnFrame.and₂;
+    | and₃ => apply ValidOnFrame.and₃; simpa;
+    | or₁ => apply ValidOnFrame.or₁;
+    | or₂ => apply ValidOnFrame.or₂;
+    | or₃ => apply ValidOnFrame.or₃; simpa;
+    | neg_equiv => apply ValidOnFrame.neg_equiv;
+    | mdp ihpq ihp =>
+      apply ValidOnFrame.mdp hRefl;
+      assumption;
+      assumption;
+    | eaxm h =>
+      obtain ⟨_, rfl⟩ := h;
+      apply ValidOnFrame.efq;
+  nonempty := by
+    use { World := PUnit, Rel := λ _ _ => True };
+    simp [Transitive, Reflexive];
+
+abbrev _root_.LO.Kripke.TransitiveReflexiveFrameClass : FrameClass := 𝔽((λ F => Transitive F ∧ Reflexive F))
+
+
+instance : Sound (𝐈𝐧𝐭 : DeductionParameter α) TransitiveReflexiveFrameClass# :=
+  LO.Kripke.instSoundOfCharacterizability (characterizability := Kripke.Characteraizable_Int)
+
+instance Characteraizable_Cl : Kripke.Characteraizable 𝔽((𝐂𝐥 : DeductionParameter α)) (λ F => Transitive F ∧ Reflexive F ∧ Extensive F) where
+  characterize := by
+    simp [System.theory];
+    intro F hTrans hRefl hExt p hp;
+    induction hp using Deduction.rec! with
+    | verum => apply ValidOnFrame.verum;
+    | imply₁ => apply ValidOnFrame.imply₁; simpa;
+    | imply₂ => apply ValidOnFrame.imply₂; simpa; simpa;
+    | and₁ => apply ValidOnFrame.and₁;
+    | and₂ => apply ValidOnFrame.and₂;
+    | and₃ => apply ValidOnFrame.and₃; simpa;
+    | or₁ => apply ValidOnFrame.or₁;
+    | or₂ => apply ValidOnFrame.or₂;
+    | or₃ => apply ValidOnFrame.or₃; simpa;
+    | neg_equiv => apply ValidOnFrame.neg_equiv;
+    | mdp ihpq ihp =>
+      apply ValidOnFrame.mdp hRefl;
+      assumption;
+      assumption;
+    | eaxm h =>
+      rcases h with (⟨_, rfl⟩ | ⟨_, rfl⟩);
+      . apply ValidOnFrame.efq;
+      . apply ValidOnFrame.lem; simpa;
+  nonempty := by
+    use { World := PUnit, Rel := λ _ _ => True };
+    simp [Transitive, Reflexive, Extensive];
+
+abbrev _root_.LO.Kripke.TransitiveReflexiveExtensiveFrameClass : FrameClass := 𝔽((λ F => Transitive F ∧ Reflexive F ∧ Extensive F))
+
+instance : Sound (𝐂𝐥 : DeductionParameter α) TransitiveReflexiveExtensiveFrameClass# :=
+  LO.Kripke.instSoundOfCharacterizability (characterizability := Kripke.Characteraizable_Cl)
+
+end Kripke
+
+
+namespace Kripke
+
+def AxiomSetFrameClass (Ax : AxiomSet α) : FrameClass.Dep α := { (F : Frame.Dep α) | F ⊧* Ax }
 notation "𝔽(" Ax ")" => Kripke.AxiomSetFrameClass Ax
+
+def FrameClassOf (Λ : DeductionParameter α) : FrameClass.Dep α := { (F : Frame.Dep α) | F ⊧* System.theory Λ }
+
+/-
 
 def AxiomSetFiniteFrameClass (Ax : AxiomSet α) : FiniteFrameClass' α := { (F : FiniteFrame' α) | F.toFrame' ⊧* Ax }
 notation "𝔽ꟳ(" Ax ")" => Kripke.AxiomSetFiniteFrameClass Ax
+-/
 
 variable {Ax : AxiomSet α}
 
-lemma validOnAxiomSetFrameClass_axiom (h : p ∈ Ax) : 𝔽(Ax) ⊧ p := by intro F hF; exact hF.realize h;
+lemma validOnAxiomSetFrameClass_axiom (h : p ∈ Ax) : 𝔽(Ax) ⊧ p := by
+  intro F hF;
+  apply hF.realize;
+  simpa;
 
-class Definability (Ax : AxiomSet α) (P : FrameProperty) where
-  defines : ∀ (F : Frame' α), F ⊧* Ax ↔ P F
+class Definability (Ax : AxiomSet α) (P : Frame → Prop) where
+  defines : ∀ (F : Frame.Dep α), F# ⊧* Ax ↔ P F
 
-instance Definability.instUnion (definability₁ : Definability Ax₁ P₁) (definability₂ : Definability Ax₂ P₂) : Definability (Ax₁ ∪ Ax₂) (λ F => P₁ F ∧ P₂ F) where
+instance Definability.instUnion
+  (definability₁ : Definability Ax₁ P₁)
+  (definability₂ : Definability Ax₂ P₂)
+  : Definability (Ax₁ ∪ Ax₂) (λ F => P₁ F ∧ P₂ F) where
   defines F := by
     constructor;
     . intro h;
@@ -346,21 +629,30 @@ instance Definability.instUnion (definability₁ : Definability Ax₁ P₁) (def
       . apply Definability.defines F |>.mpr h.1;
       . apply Definability.defines F |>.mpr h.2;
 
-lemma iff_definability_memAxiomSetFrameClass (definability : Definability Ax P) : ∀ {F : Frame' α}, F ∈ 𝔽(Ax) ↔ P F := by
+lemma iff_definability_memAxiomSetFrameClass (definability : Definability Ax P) : ∀ {F}, F ∈ 𝔽(Ax) ↔ P F := by
   apply Definability.defines;
 
+/-
 class FiniteDefinability (Ax : AxiomSet α) (P : FiniteFrameProperty) where
   defines : ∀ (F : FiniteFrame' α), F.toFrame' ⊧* Ax ↔ P F
 
 lemma iff_definability_memAxiomSetFiniteFrameClass (definability : FiniteDefinability Ax P) : ∀ {F : FiniteFrame' α}, F ∈ 𝔽ꟳ(Ax) ↔ P F := by
   apply definability.defines;
+-/
+
+
+instance EFQ_definability : Kripke.Definability (α := α) 𝗘𝗙𝗤 (λ _ => True) where
+  defines F := by simp; intros; apply ValidOnFrame.efq
+
+instance : (𝔽(𝗘𝗙𝗤) : FrameClass.Dep α).Nonempty := by
+  use { World := PUnit, Rel := λ x y => x ≤ y };
+  apply iff_definability_memAxiomSetFrameClass EFQ_definability |>.mpr;
+  trivial;
 
 end Kripke
 
-instance AxiomSet.EFQ.definability : Definability (α := α) 𝗘𝗙𝗤 (λ _ => True) where
-  defines F := by simp; intros; apply ValidOnFrame.efq
-
-instance AxiomSet.EFQ.nonempty : FrameClass.IsNonempty (𝔽(𝗘𝗙𝗤) : FrameClass' α) where
+/-
+instance AxiomSet.EFQ.nonempty : (𝔽(𝗘𝗙𝗤) : FrameClass.Dep α).Nonempty where
   nonempty := by
     existsi { World := PUnit, Rel := λ x y => x ≤ y };
     apply iff_definability_memAxiomSetFrameClass AxiomSet.EFQ.definability |>.mpr;
@@ -374,5 +666,6 @@ instance AxiomSet.EFQ.instUnionNonempty [FrameClass.IsNonempty 𝔽(Ax)] (defina
     existsi F;
     apply iff_definability_memAxiomSetFrameClass (AxiomSet.EFQ.instDefinabilityUnion definability) |>.mpr;
     apply iff_definability_memAxiomSetFrameClass definability |>.mp hF;
+-/
 
 end LO.Propositional.Superintuitionistic
